isabelle/Distinct_Elems_While.thy
@@ -1,0 +1,34 @@
+theory Distinct_Elems_While
+
+imports
+  Probabilistic_While.While_SPMF
+  CVM.Distinct_Elems_Algo
+
+begin
+
+context with_threshold
+begin
+
+term loop_spmf.while
+
+definition step_while :: \<open>'a \<Rightarrow> 'a state \<Rightarrow> 'a state spmf\<close> where
+  \<open>step_while x state \<equiv> do {
+    insert_x_into_chi \<leftarrow> bernoulli_pmf <| 1 / 2 ^ (state_k state);
+
+    let chi = (state
+      |> state_chi
+      |> if insert_x_into_chi
+        then insert x
+        else Set.remove x);
+
+    state\<lparr>state_chi := chi\<rparr>
+      |> loop_spmf.while (\<lambda> state. card (state_chi state) \<ge> threshold)
+        (\<lambda> state. do {
+          keep_in_chi :: 'a \<Rightarrow> bool \<leftarrow>
+            prod_pmf chi \<lblot>bernoulli_pmf <| 1 / 2\<rblot>;
+
+          undefined }) }\<close>
+
+end
+
+end
